make opaque insert function

lib/sequences.dfy
@@ -52,15 +52,13 @@ module Sequences {
     else FoldLeft(f, f(init, run[0]), run[1..])
   }
 
-  /*
-  function method insert<A>(s: seq<A>, a: A, pos: int)
-  requires 0 <= pos <= |s|
-  ensures |insert(s,a,pos)| == |a| + 1
-  ensures forall i :: 0 <= i < pos ==> insert(s, a, pos)[i] == s[i]
-  ensures forall i :: pos < i < |s| ==> insert(s, a, pos)[i+1] == s[i]
-  ensures insert(s, a, pos)[pos] == a
+  function method {:opaque} insert<A>(s: seq<A>, a: A, pos: int) : seq<A>
+  requires 0 <= pos <= |s|;
+  ensures |insert(s,a,pos)| == |s| + 1;
+  ensures forall i :: 0 <= i < pos ==> insert(s, a, pos)[i] == s[i];
+  ensures forall i :: pos <= i < |s| ==> insert(s, a, pos)[i+1] == s[i];
+  ensures insert(s, a, pos)[pos] == a;
   {
-    return s[..pos] + [a] + s[pos..];
+    s[..pos] + [a] + s[pos..]
   }
-  */
 }
